permit calls to builtins in L10 calldag

Calldag.v
@@ -1,8 +1,13 @@
-From Coq Require Import String Arith.
-From Vyper Require Import Config.
+From Coq Require Import String List ListSet Arith NArith.
+From Vyper Require Map FSet MapSig.
+From Vyper Require Import Config Graph.Depthmap.
 
-Record generic_calldag {C: VyperConfig} (decl_type: Type) (callset: decl_type -> string_set) := {
-  cd_decls: string_map decl_type;
+Record generic_calldag {C: VyperConfig} 
+                       {Decl: Type}
+                       (callset: Decl -> string_set)
+                       (may_call_undeclared: bool)
+:= {
+  cd_decls: string_map Decl;
   cd_depthmap: string -> option nat;
   cd_depthmap_ok:
     let _ := string_map_impl in
@@ -16,20 +21,23 @@ Record generic_calldag {C: VyperConfig} (decl_type: Type) (callset: decl_type ->
               let _ := string_set_impl in
               FSet.for_all (callset decl)
                            (fun callee => match cd_depthmap callee with
-                                          | None => false
+                                          | None => may_call_undeclared
                                           | Some y => y <? x
                                           end)
                = true
             end
       end;
 }.
-Arguments cd_decls {C decl_type callset}.
-Arguments cd_depthmap {C decl_type callset}.
-Arguments cd_depthmap_ok {C decl_type callset}.
+Arguments cd_decls       {C Decl callset may_call_undeclared}.
+Arguments cd_depthmap    {C Decl callset may_call_undeclared}.
+Arguments cd_depthmap_ok {C Decl callset may_call_undeclared}.
 
 (* This is for compatibility with an older definition via cd_declmap. *)
-Definition cd_declmap {C: VyperConfig} {decl_type: Type} {callset: decl_type -> string_set}
-                      (d: generic_calldag decl_type callset)
+Definition cd_declmap {C: VyperConfig}
+                      {Decl: Type}
+                      {callset: Decl -> string_set}
+                      {may_call_undeclared: bool}
+                      (d: generic_calldag callset may_call_undeclared)
 := let _ := string_map_impl in
    Map.lookup (cd_decls d).
 
@@ -37,30 +45,32 @@ Definition cd_declmap {C: VyperConfig} {decl_type: Type} {callset: decl_type -> 
   A functional context is the result of looking up a function by name in a calldag.
  *)
 Record fun_ctx {C: VyperConfig}
-               {decl_type: Type}
-               {decl_callset: decl_type -> string_set}
-               (cd: generic_calldag decl_type decl_callset)
+               {Decl: Type}
+               {decl_callset: Decl -> string_set}
+               {may_call_undeclared: bool}
+               (cd: generic_calldag decl_callset may_call_undeclared)
                (bound: nat) := {
   fun_name: string;
   fun_depth: nat;
   fun_depth_ok: cd_depthmap cd fun_name = Some fun_depth;
-  fun_decl: decl_type;
+  fun_decl: Decl;
   fun_decl_ok: cd_declmap cd fun_name = Some fun_decl;
   fun_bound_ok: fun_depth <? bound = true;
 }.
-Arguments fun_name     {C _ _ _ _}.
-Arguments fun_depth    {C _ _ _ _}.
-Arguments fun_depth_ok {C _ _ _ _}.
-Arguments fun_decl     {C _ _ _ _}.
-Arguments fun_decl_ok  {C _ _ _ _}.
-Arguments fun_bound_ok {C _ _ _ _}.
+Arguments fun_name     {C _ _ _ _ _}.
+Arguments fun_depth    {C _ _ _ _ _}.
+Arguments fun_depth_ok {C _ _ _ _ _}.
+Arguments fun_decl     {C _ _ _ _ _}.
+Arguments fun_decl_ok  {C _ _ _ _ _}.
+Arguments fun_bound_ok {C _ _ _ _ _}.
 
 Local Lemma make_fun_ctx_helper {C: VyperConfig}
-                                {decl_type: Type}
-                                {decl_callset: decl_type -> string_set}
-                                {cd: generic_calldag decl_type decl_callset}
+                                {Decl: Type}
+                                {decl_callset: Decl -> string_set}
+                                {may_call_undeclared: bool}
+                                {cd: generic_calldag decl_callset may_call_undeclared}
                                 {name: string}
-                                {d: decl_type}
+                                {d: Decl}
                                 (Ed: cd_declmap cd name = Some d)
                                 (Edepth: cd_depthmap cd name = None):
   False.
@@ -72,9 +82,10 @@ Qed.
 
 (** Create a function context from scratch (meaning that there's no pre-existing bound). *)
 Definition make_fun_ctx_and_bound {C: VyperConfig}
-                                  {decl_type: Type}
-                                  {decl_callset: decl_type -> string_set}
-                                  (cd: generic_calldag decl_type decl_callset)
+                                  {Decl: Type}
+                                  {decl_callset: Decl -> string_set}
+                                  {may_call_undeclared: bool}
+                                  (cd: generic_calldag decl_callset may_call_undeclared)
                                   (name: string)
 : option { bound: nat & fun_ctx cd bound }
 := match cd_declmap cd name as maybe_d return _ = maybe_d -> _ with
@@ -196,3 +207,283 @@ destruct (Map.alist_lookup KeyEqDec (Map.items m) key); inversion E; subst.
 }
 now rewrite Map.of_alist_ok.
 Qed.
+
+(**************************************************************************************************)
+
+(** Convert a list of declarations into a dictionary.
+    A duplicate declaraton name will result in an error.
+ *)
+Fixpoint make_declmap {C: VyperConfig} {Decl: Type} (get_decl_name: Decl -> string) (decls: list Decl)
+: string + string_map Decl
+:= let _ := string_map_impl in
+   match decls with
+   | nil => inr Map.empty
+   | (h :: t)%list =>
+       match make_declmap get_decl_name t with
+       | inl err => inl err
+       | inr m => let name := get_decl_name h in
+                  match Map.lookup m name with
+                  | Some _ => inl ("duplicate name: " ++ name)%string
+                  | None => inr (Map.insert m name h)
+                  end
+       end
+   end.
+
+(** Same as [make_declmap] but doesn't check for duplicates. *)
+Fixpoint make_declmap_unchecked {C: VyperConfig} {Decl: Type}
+                                (get_decl_name: Decl -> string)
+                                (decls: list Decl)
+: string_map Decl
+:= let _ := string_map_impl in
+   match decls with
+   | nil => Map.empty
+   | (h :: t)%list => Map.insert (make_declmap_unchecked get_decl_name t) (get_decl_name h) h
+   end.
+
+(** An alternative implementation of [make_declmap_unchecked]. *)
+Lemma make_declmap_unchecked_alt {C: VyperConfig} {Decl: Type}
+                                 (get_decl_name: Decl -> string)
+                                 (decls: list Decl):
+  make_declmap_unchecked get_decl_name decls
+   =
+  let _ := string_map_impl in
+  Map.of_alist (map (fun d => (get_decl_name d, d)) decls).
+Proof.
+induction decls. { easy. }
+cbn in *. now rewrite IHdecls.
+Qed.
+
+Lemma make_declmap_nodup {C: VyperConfig} {Decl: Type}
+                         (get_decl_name: Decl -> string)
+                         (decls: list Decl)
+                         (Ok: NoDup (List.map get_decl_name decls)):
+  make_declmap get_decl_name decls = inr (make_declmap_unchecked get_decl_name decls).
+Proof.
+induction decls. { easy. }
+cbn in Ok. rewrite NoDup_cons_iff in Ok. destruct Ok as (NotIn, NoDupTail).
+cbn. rewrite (IHdecls NoDupTail).
+rewrite make_declmap_unchecked_alt. cbn.
+rewrite Map.of_alist_ok.
+rewrite Map.alist_lookup_not_in. { trivial. }
+now rewrite map_map.
+Qed.
+
+(***************************************************************************)
+
+Definition has {C: VyperConfig} {Value: Type}
+               (m: string_map Value)
+               (key: string)
+: bool
+:= let _ := string_map_impl in
+   match Map.lookup m key with
+   | Some _ => true
+   | None => false
+   end.
+
+Definition declared_name {C: VyperConfig} {Decl: Type} (declmap: string_map Decl)
+: Type
+:= {name: string | has declmap name = true}.
+
+Lemma declared_name_irrel {C: VyperConfig} {Decl: Type} (declmap: string_map Decl)
+                          (a b: declared_name declmap)
+                          (E: proj1_sig a = proj1_sig b):
+  a = b.
+Proof.
+destruct a as (a_name, a_ok).
+destruct b as (b_name, b_ok).
+cbn in E. subst.
+enough (a_ok = b_ok) by now subst.
+apply Eqdep_dec.eq_proofs_unicity.
+decide equality.
+Qed.
+
+Local Lemma decl_of_declared_name_helper {C: VyperConfig} {Decl: Type} {declmap: string_map Decl}
+                                         (query: declared_name declmap)
+                                         (E: let _ := string_map_impl in
+                                             Map.lookup declmap (proj1_sig query) = None)
+                                         (ok: has declmap (proj1_sig query) = true):
+  False.
+Proof.
+unfold has in ok. cbn in E.
+now destruct Map.lookup.
+Qed.
+
+Definition decl_of_declared_name {C: VyperConfig} {Decl: Type} {declmap: string_map Decl}
+                                 (query: declared_name declmap)
+: Decl
+:= let _ := string_map_impl in
+   match Map.lookup declmap (proj1_sig query) as result return _ = result -> _ with
+   | Some x => fun _ => x
+   | None => fun E => False_rect _ (decl_of_declared_name_helper query E (proj2_sig query))
+   end eq_refl.
+
+Definition Calls {C: VyperConfig} {Decl: Type} {declmap: string_map Decl}
+                 (callset: Decl -> string_set)
+                 (caller callee: declared_name declmap)
+: Prop
+:= let _ := string_set_impl in
+   FSet.has (callset (decl_of_declared_name caller)) (proj1_sig callee) = true.
+
+(** Build a list of dependent pairs from a list and a Forall condition. *)
+Fixpoint list_exist {T: Type} {P: T -> Prop} {l: list T} (F: Forall P l)
+: list {x: T | P x}
+:= match l as l' return l = l' -> _ with
+   | nil => fun _ => nil
+   | h :: t => fun E => let F': Forall P (h :: t) := eq_ind l (Forall P) F (h :: t) E in
+                        exist _ h (Forall_inv F') :: list_exist (Forall_inv_tail F')
+   end eq_refl.
+
+Lemma list_exist_in {T: Type} {P: T -> Prop} {l: list T} (F: Forall P l)
+                    (Irrel: forall (a b: {x: T | P x}),
+                              proj1_sig a = proj1_sig b -> a = b)
+                    (x: T) (Px: P x):
+  In x l <-> In (exist _ x Px) (list_exist F).
+Proof.
+induction l as [|h]. { easy. }
+cbn. split; intro H; case H; clear H; intro H.
+{ left. subst. now apply Irrel. }
+{ right. now apply IHl. }
+{ left. now inversion H. }
+right. now apply IHl in H.
+Qed.
+
+Definition all_names {C: VyperConfig} {Decl: Type} (declmap: string_map Decl)
+:= let _ := string_map_impl in
+   map fst (Map.items declmap).
+
+Lemma all_names_ok {C: VyperConfig} {Decl: Type} (declmap: string_map Decl) (name: string):
+  In name (all_names declmap)  <->  has declmap name = true.
+Proof.
+unfold has. unfold all_names.
+assert (ItemsOk := let _ := string_map_impl in Map.items_ok declmap name).
+rewrite ItemsOk. clear ItemsOk.
+remember (Map.items declmap) as l. clear Heql. induction l as [|head]. { easy. }
+destruct head as (key, value). cbn.
+destruct (string_dec name key) as [E|NE]. { symmetry in E. tauto. }
+assert (NE': key <> name). { intro H. symmetry in H. contradiction. }
+tauto.
+Qed.
+
+Lemma all_declared_names_helper {C: VyperConfig} {Decl: Type} (declmap: string_map Decl):
+  let _ := string_map_impl in
+  Forall (fun name => has declmap name = true) (all_names declmap).
+Proof.
+rewrite Forall_forall. intros name. apply all_names_ok.
+Qed.
+
+Definition all_declared_names {C: VyperConfig} {Decl: Type} (declmap: string_map Decl)
+: list (declared_name declmap)
+:= list_exist (all_declared_names_helper declmap).
+
+Lemma all_declared_names_ok {C: VyperConfig} {Decl: Type} (declmap: string_map Decl)
+                            (d: declared_name declmap):
+  In d (all_declared_names declmap).
+Proof.
+destruct d as (name, is_declared).
+apply (list_exist_in (all_declared_names_helper declmap)
+                     (declared_name_irrel declmap)).
+unfold all_names.
+unfold has in is_declared.
+assert (ItemsOk := let _ := string_map_impl in Map.items_ok declmap name).
+destruct (Map.lookup declmap name). 2:{ discriminate. }
+remember (Map.items declmap) as l. clear Heql. induction l as [|head]. { easy. }
+destruct head as (head_name, head_decl).
+cbn in *.
+destruct string_dec. { left. now symmetry. }
+right. exact (IHl ItemsOk).
+Qed.
+
+Definition declset {C: VyperConfig} {Decl: Type} (declmap: string_map Decl)
+: string_set
+:= let _ := string_set_impl in
+   let _ := string_map_impl in
+   FSet.from_list (map fst (Map.items declmap)).
+
+(** The list of called functions but restricted to the actually declared symbols
+    (not actually declared functions because with parameterized [Decl]
+    we have no way to distinguish function declarations from other declarations)
+ *)
+Definition restricted_call_list {C: VyperConfig} {Decl: Type}
+                                {declmap: string_map Decl}
+                                (callset: Decl -> string_set)
+                                (d: declared_name declmap)
+: list string
+:= let _ := string_set_impl in
+   set_inter string_dec (FSet.to_list (callset (decl_of_declared_name d))) (all_names declmap).
+
+Lemma restricted_call_list_nodup {C: VyperConfig} {Decl: Type}
+                                 (declmap: string_map Decl)
+                                 (callset: Decl -> string_set)
+                                 (d: declared_name declmap):
+  NoDup (restricted_call_list callset d).
+Proof.
+apply set_inter_nodup.
+{ apply FSet.to_list_nodup. }
+apply Map.items_nodup.
+Qed.
+
+Lemma restricted_call_list_all_declared {C: VyperConfig} {Decl: Type}
+                                        {declmap: string_map Decl}
+                                        (callset: Decl -> string_set)
+                                        (d: declared_name declmap):
+  Forall (fun name => has declmap name = true)
+         (restricted_call_list callset d).
+Proof.
+rewrite Forall_forall. intros name H.
+unfold restricted_call_list in H.
+apply set_inter_elim2 in H.
+revert name H. rewrite<- Forall_forall.
+apply all_declared_names_helper.
+Qed.
+
+Definition declared_call_list {C: VyperConfig} {Decl: Type}
+                              {declmap: string_map Decl}
+                              (callset: Decl -> string_set)
+                              (d: declared_name declmap)
+: list (declared_name declmap)
+:= list_exist (restricted_call_list_all_declared callset d).
+
+
+Lemma declared_call_list_ok {C: VyperConfig} {Decl: Type}
+                            {declmap: string_map Decl}
+                            (callset: Decl -> string_set)
+                            (a b: declared_name declmap):
+  In b (declared_call_list callset a)  <->  Calls callset a b.
+Proof.
+unfold Calls. unfold declared_call_list.
+destruct b as (b_name, b_ok).
+rewrite<- (list_exist_in (restricted_call_list_all_declared callset a)
+            (declared_name_irrel declmap)).
+unfold restricted_call_list. cbn.
+rewrite FSet.has_to_list.
+remember (FSet.to_list (callset (decl_of_declared_name a))) as l. destruct Heql.
+rewrite ListSet2.set_mem_true.
+rewrite set_inter_iff.
+enough (In b_name (all_names declmap)) by tauto.
+now apply all_names_ok.
+Qed.
+
+Definition make_depthmap {C: VyperConfig} {Decl: Type}
+                         (declmap: string_map Decl)
+                         (callset: Decl -> string_set)
+: Cycle.t (Calls callset) +
+  { f: declared_name declmap -> N |
+      forall a b : declared_name declmap,
+        Calls callset a b -> (f b < f a)%N }
+:= cycle_or_depthmap (Calls callset) (all_declared_names declmap) (all_declared_names_ok declmap)
+     (MapSig.instance
+       (string_map_impl ({start : declared_name declmap & Path.t (Calls callset) start} * N)))
+     (declared_call_list callset)
+     (declared_call_list_ok callset).
+
+Definition cycle_error_message {C: VyperConfig} {Decl: Type}
+                               (declmap: string_map Decl)
+                               {callset: Decl -> string_set}
+                               (cycle: Cycle.t (@Calls C Decl declmap callset))
+: string
+:= let fix path_to_string {v: declared_name declmap} (p: Path.t (Calls callset) v)
+       := match p with
+          | Path.Nil _ => proj1_sig v
+          | Path.Cons _ _ rest => (proj1_sig v ++ " -> " ++ path_to_string rest)%string
+          end
+   in ("recursion is not allowed but a call cycle is detected: " ++ path_to_string (Cycle.path cycle)).
